iris_system/sWorld.v
@@ -1,58 +1,75 @@
 From stdpp Require Import coPset gmap namespaces.
-Require Import sflib.
 From iris Require Import bi.big_op.
 Require Import Coq.Logic.ClassicalEpsilon.
-Require Export World.
+Require Export Coqlib own SRF sProp World.
 
 (* TODO : move these to separate files *)
 Local Notation univ_id := positive.
 Local Notation level := nat.
 
+(* Syntactic invariants *)
+Variant inv_shape : Type :=
+| _ownI (u : univ_id) (i : positive)
+| _ownI_auth (u : univ_id) (keys : gmap positive unit)
+| _wsat_auth (u : univ_id).
+
+Local Definition inv_degree (s : inv_shape) (sProp : Type) : Type :=
+  match s with
+  | _ownI u i => fin 1
+  | _ownI_auth u keys => positive
+  | _wsat_auth u => fin 0
+  end.
+
+Global Instance inv_syntax : PF.t := {
+  shp := inv_shape;
+  deg := inv_degree;
+}.
+(* TODO : find a way to construct gmap of SRFSyns from syn : pos → SRFSyn.t *)
+(* Invariant interpretations *)
+Local Definition inv_interp_aux `{α : SRFCons.t, !subG Γ Σ, !invGS Σ Γ} n (s : inv_shape) :
+    (inv_degree s (SRFSyn.t_prev n) → SRFSyn.t n) → (inv_degree s (SRFSyn.t_prev n) → iProp Σ)
+    → iProp Σ :=
+  match s with
+  | _ownI u i => λ syn _, ownI u n i (syn 0%fin)
+  | _ownI_auth u keys => λ syn _, ownI_auth u n (map_imap (λ k v, Some (syn k)) keys)
+  | _wsat_auth u => λ _ _, wsat_auth u n
+  end.
+
+Global Instance inv_interp `{α : SRFCons.t, !subG Γ Σ, !invGS Σ Γ} : @SRFIntpM.t (@domain Σ) α _ :=
+  inv_interp_aux.
+
 Section syn_inv.
-  Context `{!CtxSL.t Σ Γ α β τ, !invGSΓ Γ}.
+  Context `{!CtxSL.t Σ Γ α β τ, !invGS Σ Γ, !SRFIntp.inG _ α inv_interp β}.
+  Local Definition a : SRFDom.t := domain Σ.
+  Local Existing Instance a.
+  Local Existing Instances inv_preΣ inv_preΓ invGS_I invGS_E invGS_D.
 
-  Variant syn_inv_shape : Type :=
-  | _ownI (u : univ_id) (i : positive)
-  | _ownI_auth (u : univ_id) (keys : gset positive) (* TODO : gsets? *)
-  | _wsat_auth (u : univ_id) (n)
-  (* | _free_worlds (u : univ_id) (b : level) *)
-  (* | _empty_universes (eu : univ_id) *)
-  .
+  Local Definition syn_ownI u n i (p : SRFSyn.t n) : SRFSyn.t n :=
+    ⟨ _ownI u i, λ _, p ⟩.
+  Local Definition syn_ownI_auth u n (I : gmap positive (SRFSyn.t n)) : SRFSyn.t n :=
+    ⟨ _ownI_auth u (gset_to_gmap tt (dom I)), λ i, or_else (I !! i) emp%SRF⟩.
+  Local Definition syn_wsat_auth u n : SRFSyn.t n :=
+    ⟨ _wsat_auth u, λ e, match e with end ⟩.
 
-  Definition inv_degree (s : inv_shape) (sProp : Type) : Type :=
-    match s with
-    (* | _OwnI u i => fin 1
-    | _OwnI_auth u keys => positive
-    | _free_worlds u b => fin 0
-    | _empty_universes u => fin 0 *)
-    | _inv u n N p => fin 0
-    | _wsats u n E => fin 0
+  Local Definition syn_ownE (u : univ_id) n (E : coPset) : SRFSyn.t n :=
+    <own> enabled_name (ownER u E).
+  Local Definition syn_ownD (u : univ_id) n (D : gset positive) : SRFSyn.t n :=
+    <own> disabled_name (ownDR u D).
+  Local Definition syn_ownD_auth (u : univ_id) n : SRFSyn.t n :=
+    (∃ D : τ{⇣gset positive}, <own> disabled_name (ownD_authR u D))%SRF.
+
+  Local Definition syn_inv_satall u n (I : gmap positive (SRFSyn.t n)) : SRFSyn.t n :=
+    ([∗ n map] i ↦ p ∈ I, (p ∗ syn_ownD u n {[i]}) ∨ syn_ownE u n {[i]})%SRF.
+  Local Definition syn_wsat u n : SRFSyn.t (S n) :=
+    (∃ I : τ{ST.gmapT Φ}, (⤉ syn_ownI_auth u n I) ∗ (⤉ syn_inv_satall u n I))%SRF.
+  (* wsat_auth u (S n) ∗ ownE u E ∗ ownD_auth u ∗ [∗ list] n ∈ (seq 0 (S n)), wsat u n. *)
+  Local Fixpoint syn_wsats_aux u n : SRFSyn.t n :=
+    match n with
+    | O => emp%SRF
+    | S n' => syn_wsat u n' ∗ ⤉ syn_wsats_aux u n'
     end.
-
-  Global Instance inv_syntax : PF.t := {
-      shp := inv_shape;
-      deg := inv_degree;
-    }.
-
-  Definition inv_interp_aux n (s : inv_shape)
-      : (inv_degree s (SRFSyn.t_prev n) → SRFSyn.t n) → (inv_degree s (SRFSyn.t_prev n) → iProp Σ)
-        → iProp Σ :=
-    match s with
-    (* | _OwnI u i => fun syn _ =>
-        OwnI u n i (syn 0%fin)
-    | _OwnI_auth u keys => fun syn _ =>
-        OwnI_auth u n (list_to_map ((fun i => (i, syn i)) <$> keys))
-    | _free_worlds u b => fun _ _ =>
-        free_worlds u b
-    | _empty_universes eu => fun _ _ =>
-        empty_universes eu *)
-    | _inv u n N p => λ _ _, inv u n N p
-    | _wsats u n E => λ _ _, wsats u n E
-    end.
-
-  Global Instance inv_interp : SRFIntpM.t := inv_interp_aux.
-
-  Context `{_W3 : @SRFIntp.inG SL.domain inv_syntax α inv_interp β}.
+  Local Definition syn_wsats u n (E : coPset) : SRFSyn.t n :=
+    syn_wsat_auth u n ∗ syn_ownE u n E ∗ syn_ownD_auth u n ∗ syn_wsats_aux u n.
 
   (* Definition OwnI u n i (p : SRFSyn.t n) : SRFSyn.t n := *)
     (* ⟨ _OwnI u i, fun _ => p ⟩%SRF. *)
@@ -74,10 +91,10 @@ Section syn_inv.
     (* ([∗ n map] i ↦ p ∈ I, (p ∗ OwnD u {[i]}) ∨ OwnE u {[i]})%SRF. *)
   (* Definition wsat u n : SRFSyn.t (S n) := *)
     (* (∃ I : τ{ST.gmapT Φ}, (⤉ OwnI_auth u n I) ∗ (⤉ inv_satall u n I))%SRF. *)
-  Definition syn_wsats (u : univ_id) (n : level) (E : coPset) : SRFSyn.t n :=
+  (* Definition syn_wsats (u : univ_id) (n : level) (E : coPset) : SRFSyn.t n :=
     ⟨ _wsats u n E, λ e, match e with end ⟩%SRF.
   Definition syn_inv (u : univ_id) (n : level) (N : namespace) (p : SRFSyn.t n) : SRFSyn.t n :=
-    ⟨ _inv u n N p, λ e, match e with end ⟩%SRF.
+    ⟨ _inv u n N p, λ e, match e with end ⟩%SRF. *)
   (* Definition syn_fupd u b (E1 E2 : coPset) (P : iProp Σ) : SRFSyn.t n :=
     syn_wsats u b E1 ==∗ (syn_wsats u b E2 ∗ P) *)
 
@@ -98,139 +115,98 @@ Section syn_inv.
     (* wsats u b ∗ OwnE u E ∗ ownD_auth u ∗ free_universes. *)
   (* Definition closed_universe u b E : SRFSyn.t b := *)
     (* used_worlds u b E ∗ free_worlds u b. *)
-  (* Definition inv u (n : level) (N : namespace) p := *)
-    (* (∃ i : τ{⇣positive}, ⌜i ∈ (↑N : coPset)⌝ ∧ OwnI u n i p)%SRF. *)
-  (* Definition FUpd u b (A : SRFSyn.t b) (E1 E2 : coPset) (P : SRFSyn.t b) : SRFSyn.t b := *)
-    (* A ∗ used_worlds u b E1 -∗ |==> (A ∗ used_worlds u b E2 ∗ P). *)
-  Context (p : SRFSyn.t 0).
-  Check (syn_inv 1 0 nil (syn_wsats 1 0 ⊤)).
+  Local Definition syn_inv_def (u : univ_id) (n : level) (N : namespace) p :=
+    (∃ i : τ{⇣positive}, ⌜i ∈ (↑N : coPset)⌝ ∧ syn_ownI u n i p)%SRF.
+  Local Definition syn_inv_aux : seal (@syn_inv_def). Proof. by eexists. Qed.
+  Definition syn_inv := syn_inv_aux.(unseal).
+  Local Definition syn_inv_eq : @syn_inv = @syn_inv_def := syn_inv_aux.(seal_eq).
+
+  Local Definition syn_fupd_def u b (E1 E2 : coPset) (P : SRFSyn.t b) : SRFSyn.t b :=
+    syn_wsats u b E1 ==∗ (syn_wsats u b E2 ∗ P).
+  Local Definition syn_fupd_aux : seal (@syn_fupd_def). Proof. by eexists. Qed.
+  Definition syn_fupd := syn_fupd_aux.(unseal).
+  Local Definition syn_fupd_eq : @syn_fupd = @syn_fupd_def := syn_fupd_aux.(seal_eq).
 End syn_inv.
 
-Class sinvGS Σ Γ α β τ :=
-  { #[global] sinv_CtxSL :: CtxSL.t Σ Γ α β τ;
-    #[global] sinv_invGS :: invGS Σ Γ;
-    #[global] sinv_intpG :: @SRFIntp.inG SL.domain inv_syntax α inv_interp β
-  }.
+Class sinvGS Σ Γ α β τ := {
+  #[global] sinv_CtxSL :: CtxSL.t Σ Γ α β τ;
+  #[global] sinv_invGS :: invGS Σ Γ;
+  #[global] sinv_intpG :: @SRFIntp.inG (domain Σ) inv_syntax α inv_interp β
+}.
 
-Module WDRed. Section RED.
+(* Definition test `{!sinvGS Σ Γ α β τ} : True. Proof. exact I. Qed.
+Lemma test' : True. eapply test. Unshelve.
+{ eapply #[invΣ; invΓ]. Unshelve.  } *)
+
+Section reduction.
   Context `{!sinvGS Σ Γ α β τ}.
 
-  Lemma wsats u n E : ⟦syn_wsats u n E⟧ = wsats u n E.
-  Proof. rewrite /syn_wsats. SRF_red_all. ss. Qed.
-  Lemma inv u n N p : ⟦syn_inv u n N p⟧ = inv u n N p.
-  Proof. rewrite /syn_inv. SRF_red_all. ss. Qed.
+  Notation "'⟦' F ',' n '⟧'" := (SRFSem.t (Δ := domain Σ) n F).
+  Notation "'⟦' F '⟧'" := (SRFSem.t (Δ := domain Σ) _ F).
 
-    (* Context `{_C : Inv.t}. *)
+  Lemma ownI_auth_red u n I :
+    ⟦syn_ownI_auth u n I⟧ = ownI_auth u n I.
+  Proof.
+    SRF_red; ss.
+    f_equal. apply map_eq; intros i.
+    destruct (decide (i ∈ dom I)).
+    { rewrite map_lookup_imap lookup_gset_to_gmap //=. case_guard; ss. apply elem_of_dom in e; ss.
+      destruct (I !! i); ss; inv e.
+    }
+    { rewrite map_lookup_imap lookup_gset_to_gmap //=. case_guard; ss.
+      rewrite not_elem_of_dom_1; eauto.
+    }
+  Qed.
 
-    (* Lemma OwnI_auth u n I  : *)
-      (* SRFSem.t n (WD.OwnI_auth u n I) = OwnI_auth u n I. *)
-    (* Proof. *)
-      (* rewrite /WD.OwnI_auth. SRF_red_all. ss. *)
-      (* rewrite /OwnI_auth /OwnI_authR; do 5 f_equal. *)
-      (* apply map_eq; intros i. *)
-      (* destruct (I !! i) eqn : EI; rewrite EI. *)
-      (* { rewrite -elem_of_list_to_map. *)
-        (* rewrite elem_of_list_fmap; exists i; rewrite EI; ss; split; eauto; *)
-          (* by rewrite elem_of_elements elem_of_dom; rewrite EI. *)
-        (* eapply NoDup_fmap_fst. *)
-        (* { intros ???. rewrite !elem_of_list_fmap; ii; des; clarify. } *)
-        (* eapply NoDup_fmap_2; last by eapply NoDup_elements. *)
-        (* ii; clarify. *)
-      (* } *)
-      (* { eapply not_elem_of_list_to_map_1; intros H. *)
-        (* rewrite elem_of_list_fmap in H; des; clarify. *)
-        (* eapply elem_of_list_fmap_2 in H0; des; clarify; ss. *)
-        (* rewrite elem_of_elements elem_of_dom in H1; rewrite EI in H1; ss; inv H1. *)
-      (* } *)
-    (* Qed. *)
+  Lemma wsat_red u n : ⟦syn_wsat u n⟧ ≡ wsat u n.
+  Proof.
+    rewrite /syn_wsat /wsat; SRF_red; SL_red.
+    iSplit; iIntros "[%I H]"; SL_red.
+    { rewrite @SRFRed.lift ownI_auth_red. SRF_red. rewrite /syn_inv_satall; SL_red.
+      iExists I; iDestruct "H" as "[$ H]".
+      rewrite /inv_satall. iApply (big_sepM_mono with "H"); ss.
+      rewrite /ownD /ownE. intros k x IN; SL_red; ss.
+    }
+    { iExists I; SL_red; rewrite !@SRFRed.lift ownI_auth_red /syn_inv_satall; SL_red.
+      iDestruct "H" as "[$ H]".
+      rewrite /inv_satall. iApply (big_sepM_mono with "H"); ss.
+      rewrite /ownD /ownE. intros k x IN; SL_red; ss.
+    }
+  Qed.
 
-    (* Lemma wsat u n: *)
-      (* SRFSem.t (S n) (WD.wsat u n) ≡ wsat u n. *)
-    (* Proof. *)
-      (* rewrite /WD.wsat /wsat. SL_red. *)
-      (* rewrite bi.equiv_entails; split; ss; iIntros "[%I WD]"; SL_red; iDestruct "WD" as "[WD1 WD2]"; SL_red. *)
-      (* { SRF_red; SL_red; rewrite OwnI_auth /inv_satall; iExists I; iFrame. *)
-        (* iApply (big_sepM_impl with "WD2"); iModIntro; iIntros. rewrite /WD.OwnD /WD.OwnE; SL_red; SL_red_ownm; ss. *)
-      (* } *)
-      (* { iExists I; SL_red. SL_red. SRF_red. rewrite OwnI_auth; iFrame. *)
-        (* SL_red; rewrite /inv_satall. iApply (big_sepM_impl with "WD2"); iModIntro; iIntros. SL_red; SL_red_ownm; ss. *)
-      (* } *)
-    (* Qed. *)
+  Lemma wsats_aux_red u n : ⟦syn_wsats_aux u n⟧ ≡ ([∗ list] n ∈ (seq 0 n), wsat u n)%I.
+  Proof.
+    induction n.
+    { SRF_red; SL_red; ss. }
+    { simpl syn_wsats_aux. rewrite seq_S big_sepL_app; ss. SRF_red; ss.
+      rewrite wsat_red; SRF_red; rewrite IHn; iSplit; iIntros "[$ H]"; iFrame.
+      iDestruct "H" as "[??]"; iFrame.
+    }
+  Qed.
+  
+  Lemma wsats_red u n E : ⟦syn_wsats u n E⟧ ≡ wsats u n E.
+  Proof.
+    rewrite /syn_wsats /syn_ownE /syn_ownD_auth. SRF_red. SL_red.
+    rewrite wsats_aux_red; SRF_red; ss; rewrite /wsats /ownD_auth.
+    iSplit; iIntros "($ & $ & [%x H] & $)"; iExists x; SL_red; iFrame.
+  Qed.
 
-    (* Lemma wsats u b: *)
-      (* SRFSem.t b (WD.wsats u b) ≡ wsats u b. *)
-    (* Proof. *)
-      (* induction b; ss. *)
-      (* - SL_red. eauto. *)
-      (* - rewrite @SLRed.sepconj wsat. SRF_red. rewrite IHb. by rewrite wsats_fold. *)
-    (* Qed. *)
+  Lemma inv_red u n N p : ⟦syn_inv u n N p⟧ ≡ inv u n N p.
+  Proof.
+    rewrite syn_inv_eq /syn_inv_def. SL_red. rewrite /inv World.inv_aux.(seal_eq) /World.inv_def.
+    iSplit; iIntros "[%x H]"; iExists x; SL_red; SRF_red; ss.
+  Qed.
 
-    (* User Interface *)
-    (* Lemma used_worlds u b E : *)
-      (* SRFSem.t b (WD.used_worlds u b E) ≡ used_worlds u b E. *)
-    (* Proof. *)
-      (* SL_red; rewrite wsats; rewrite bi.equiv_entails; split. *)
-      (* { iIntros "[WSAT [E [[% D] [% U]]]]"; SL_red; iFrame. *)
-        (* by rewrite /WD.empty_universes; SRF_red; SL_red_ownm; ss; iFrame. } *)
-      (* { iIntros "[WSAT [E [[% D] [% U]]]]"; SL_red; SL_red_ownm; iFrame. *)
-        (* iSplitL "D"; [iExists D|iExists eu]; last by rewrite /WD.empty_universes; SRF_red; ss; iFrame. *)
-        (* SL_red; SL_red_ownm; iFrame. *)
-      (* } *)
-    (* Qed. *)
+  Lemma fupd_red u n E1 E2 P : ⟦syn_fupd u n E1 E2 P⟧ ≡ uPred_fupd u n E1 E2 ⟦P⟧.
+  Proof.
+    rewrite syn_fupd_eq /uPred_fupd World.uPred_fupd_aux.(seal_eq) /World.uPred_fupd_def.
+    rewrite SLRed.wand SLRed.upd wsats_red. SRF_red; ss.
+    rewrite wsats_red; done.
+  Qed.
+End reduction.
 
-    (* Lemma free_worlds u b : *)
-      (* SRFSem.t b (WD.free_worlds u b) = free_worlds u b. *)
-    (* Proof. *)
-      (* unfold free_worlds, WD.free_worlds. SRF_red. eauto. *)
-    (* Qed. *)
-
-    (* Lemma closed_universe u b E : *)
-      (* SRFSem.t b (WD.closed_universe u b E) ≡ closed_universe u b E. *)
-    (* Proof. *)
-      (* rewrite /WD.closed_universe /closed_universe @SLRed.sepconj used_worlds free_worlds; ss. *)
-    (* Qed. *)
-
-    (* Lemma inv u n N p : *)
-      (* SRFSem.t n (WD.inv u n N p) ≡ inv u n N p. *)
-    (* Proof. *)
-      (* rewrite /WD.inv /inv; SL_red; rewrite bi.equiv_entails; split; iIntros "[%x H]"; SL_red. *)
-      (* { iExists x; rewrite /WD.OwnI; SRF_red; ss. } *)
-      (* { iExists x; SL_red; rewrite /WD.OwnI; SRF_red; ss. } *)
-    (* Qed. *)
-
-    (* Lemma FUpd u b A E1 E2 P : *)
-      (* SRFSem.t b (WD.FUpd u b A E1 E2 P) ≡ FUpd u b ⟦A⟧ E1 E2 ⟦P⟧. *)
-    (* Proof. *)
-      (* Local Transparent FUpd. *)
-      (* unfold WD.FUpd, FUpd. rewrite !@SLRed.wand !@SLRed.upd @SLRed.sepconj. rewrite -> used_worlds. *)
-      (* do 2 rewrite @SLRed.sepconj. rewrite used_worlds. eauto. *)
-    (* Qed. *)
-
-  End RED.
-End WDRed.
-
-(* Global Opaque WD.used_worlds. *)
-(* Global Opaque WD.free_worlds. *)
-(* Global Opaque WD.inv. *)
-(* Global Opaque WD.FUpd. *)
-(* Global Opaque used_worlds. *)
-(* Global Opaque free_worlds. *)
-(* Global Opaque inv. *)
-(* Global Opaque FUpd. *)
-
-
-Ltac WD_red := repeat (
-                   try rewrite ! @WDRed.used_worlds;
-                   try rewrite ! @WDRed.free_worlds;
-                   try rewrite ! @WDRed.closed_universe;
-                   try rewrite ! @WDRed.inv;
-                   try rewrite ! @WDRed.FUpd
-                 ).
-
-Ltac WD_red_all := repeat (
-                       try rewrite ! @WDRed.used_worlds in *;
-                       try rewrite ! @WDRed.free_worlds in *;
-                       try rewrite ! @WDRed.closed_universe in *;
-                       try rewrite ! @WDRed.inv in *;
-                       try rewrite ! @WDRed.FUpd in *
-                     ).
+Ltac inv_red :=
+  repeat (
+    try rewrite ! inv_red;
+    try rewrite ! fupd_red
+  ).
